Veil/DSL/ActionTheory.lean
@@ -1,0 +1,218 @@
+import Veil.DSL.Base
+
+/-!
+  # Action Language
+
+  This file defines the syntax and semantics for the imperative language
+  we use to define initializers and actions.
+-/
+section Veil
+
+section Types
+/-! Our language is parametric over the state type. -/
+variable (σ : Type)
+
+/-- One-state formula -/
+@[inline] abbrev SProp := σ -> Prop
+/-- One-state formula that also talks about the return value. -/
+@[inline] abbrev RProp (ρ : Type u) := ρ → SProp σ
+/-- Two-state formula -/
+@[inline] abbrev ActProp := σ -> σ -> Prop
+
+/-  Wlp (σ : Type) (ρ : Type)    := RProp σ ρ -> SProp σ -/
+/-  Wlp (σ : Type) (ρ : Type)    := RProp σ ρ -> σ -> Prop -/
+abbrev Wlp (σ : Type) (ρ : Type) := σ -> RProp σ ρ -> Prop
+abbrev BigStep (σ : Type) (ρ : Type) := σ -> ρ -> σ -> Prop
+
+/-- Function which transforms any two-state formula into `Wlp` -/
+@[actSimp]
+def Function.toWlp (r : σ -> σ -> Prop) : Wlp σ Unit :=
+  fun s post => ∀ s', r s s' -> post () s'
+
+@[actSimp]
+def Wlp.toBigStep {σ} (act : Wlp σ ρ) : BigStep σ ρ :=
+  fun s r' s' => ¬ act s (fun r₀ s₀ => ¬ (r' = r₀ ∧ s' = s₀))
+
+@[actSimp]
+def Wlp.toActProp {σ} (act : Wlp σ ρ) : ActProp σ :=
+  fun s s' => ¬ act s (fun _ s₀ => s' ≠ s₀)
+
+@[actSimp]
+def BigStep.toWlp {σ} (act : BigStep σ ρ) : Wlp σ ρ :=
+  fun s post => ∀ r s', act s r s' -> post r s'
+
+end Types
+
+section
+
+variable {σ ρ : Type}
+
+@[actSimp]
+def Wlp.pure (r : ρ) : Wlp σ ρ := fun s post => post r s
+@[actSimp]
+def Wlp.bind (wp : Wlp σ ρ) (wp_cont : ρ -> Wlp σ ρ') : Wlp σ ρ' :=
+  fun s post => wp s (fun r s' => wp_cont r s' post)
+
+instance : Monad (Wlp σ) where
+  pure := Wlp.pure
+  bind := Wlp.bind
+
+@[actSimp]
+def Wlp.assume (rq : Prop) : Wlp σ PUnit := fun s post => rq → post () s
+-- @[actSimp]
+-- def Wlp.assert (as : Prop) : Wlp σ PUnit := fun s post => as ∧ post () s
+@[actSimp]
+def Wlp.fresh (τ : Type) : Wlp σ τ := fun s post => ∀ t, post t s
+@[actSimp]
+def Wlp.spec (req : SProp σ) (ens : σ -> RProp σ ρ) : Wlp σ ρ :=
+  fun s post => ∀ r' s', (req s -> ens s r' s') -> post r' s'
+
+
+/- alternative definition of Wlp.spec -/
+-- @[actSimp]
+-- def Wlp.spec' (req : SProp σ) (ens : σ -> RProp σ ρ) : Wlp σ ρ :=
+--   fun s post => req s ∧ (∀ r' s', ens s r' s' -> post r' s') ∨ (∀ r' s', post r' s')
+
+-- theorem check_spec_sound' [Sound act] (req : SProp σ) (ens : σ -> RProp σ ρ) :
+--   (∀ s, req s -> act s (ens s)) ->
+--   (∀ s post, Wlp.spec' req ens s post -> act s post) := by
+--   intro triple s post; unfold Wlp.spec'
+--   rintro (⟨hreq, hens⟩ | hpost)
+--   { apply Sound.impl <;> solve_by_elim }
+--   apply sound_tauto; assumption
+
+def BigStep.spec (req : SProp σ) (ens : σ -> RProp σ ρ) : BigStep σ ρ :=
+  fun s r s' => req s -> ens s r s'
+
+-- def BigStep.choice : BigStep σ ρ -> BigStep σ ρ -> BigStep σ ρ :=
+--   fun act act' s r s' => act s r s' ∨ act' s r s'
+
+/- BAD: it duplicates post -/
+-- def Wlp.choice : Wlp σ ρ -> Wlp σ ρ -> Wlp σ ρ :=
+--   fun wp wp' s post => wp s post ∨ wp' s post
+
+-- def Wlp.choice (wp : Wlp σ ρ) (wp' : Wlp σ ρ) : Wlp σ ρ :=
+--   wp.toBigStep.choice wp'.toBigStep |>.toWlp
+
+instance : MonadStateOf σ (Wlp σ) where
+  get := fun s post => post s s
+  set s' := fun _ post => post () s'
+  modifyGet := fun act s post => let (ret, s') := act s ; post ret s'
+
+class IsStateExtension (σ : semiOutParam Type) (σ' : Type) where
+  extendWith : σ -> σ' -> σ'
+  restrictTo : σ' -> σ
+
+export IsStateExtension (extendWith restrictTo)
+
+instance [IsStateExtension σ σ'] : MonadLift (Wlp σ) (Wlp σ') where
+  monadLift := fun m s post => m (restrictTo s) (fun r s' => post r (extendWith s' s))
+
+class Sound {σ ρ : Type} (act : Wlp σ ρ) where
+  inter {τ : Type} (post : τ -> RProp σ ρ) :
+    ∀ s : σ, (∀ t : τ, act s (post t)) -> act s (∀ t, post t · ·)
+  impl (post post' : RProp σ ρ) : ∀ s,
+    (∀ r s, post r s -> post' r s) -> act s post -> act s post'
+
+theorem sound_and (act : Wlp σ ρ) [Sound act] :
+  act s post -> act s post' -> act s fun r s => post r s ∧ post' r s := by
+  intro hact hact'
+  let Post := fun (b : Bool) => if b then post' else post
+  have post_eq : (fun r s => ∀ b, Post b r s) = fun r s => post r s ∧ post' r s := by
+    unfold Post; simp
+  rw [<-post_eq]; apply Sound.inter <;> simp [*, Post]
+
+theorem sound_tauto [Sound act] : (∀ r s, post r s) -> act s post := by
+  intro hpost
+  have post_eq : post = (fun _ _ => Empty -> True) := by ext; simp_all
+  rw [post_eq]; apply Sound.inter; rintro ⟨⟩
+
+theorem wlp_sound (act : Wlp σ ρ) [Sound act] :
+  ∀ s post, act.toBigStep.toWlp s post <-> act s post := by
+  intro s post; constructor
+  { unfold Wlp.toBigStep BigStep.toWlp; simp
+    intro hact
+    have post_impl : ∀ r s, (∀ r' s', ¬ post r' s' -> ¬ (r' = r ∧ s' = s)) -> post r s := by
+      intro r s impl
+      false_or_by_contra
+      specialize impl r s; apply impl <;> simp_all
+    apply Sound.impl; apply post_impl
+    apply Sound.inter; intro r'
+    apply Sound.inter; intro s'
+    by_cases postrs : post r' s'
+    { apply sound_tauto; simp_all }
+    apply Sound.impl (post := fun r₀ s₀ => r' = r₀ → ¬s' = s₀) <;> simp_all
+    false_or_by_contra
+    specialize hact _ _ ‹_›; contradiction }
+  intro hact r' s' h
+  false_or_by_contra; apply h; apply Sound.impl (post := post)
+  { intros; intro _; simp_all }
+  assumption
+
+theorem wlp_spec_to_big_step :
+  (Wlp.spec ens req).toBigStep = BigStep.spec ens req := by
+  ext s r' s'; unfold Wlp.spec BigStep.spec Wlp.toBigStep; simp
+
+theorem check_spec_sound [Sound act] (req : SProp σ) (ens : σ -> RProp σ ρ) :
+  (∀ s, req s -> act s (ens s)) ->
+  (∀ s post, Wlp.spec req ens s post -> act s post) := by
+  intro triple s post hspec
+  apply Sound.impl; apply hspec
+  have: ∀ r' s', ({t : Unit // req s} → ens s r' s') ->  (req s → ens s r' s') := by
+    intro r' s' h hreq; apply h; exact ⟨(), hreq⟩
+  apply Sound.impl; apply this
+  apply Sound.inter; rintro ⟨_, hreq⟩
+  solve_by_elim
+
+instance : Sound (Wlp.pure (σ := σ) r) where
+  inter := by simp [actSimp]
+  impl := by intros; simp_all [actSimp]
+
+instance [Sound act] [∀ r, Sound (act' r)] : Sound (Wlp.bind act act') where
+  inter := by
+    unfold Wlp.bind
+    intros τ post s hbind
+    apply Sound.impl (∀ t, act' · · <| post t) <;> solve_by_elim [Sound.inter]
+  impl := by
+    unfold Wlp.bind
+    intros post post' s hpost hbind
+    apply Sound.impl (act' · · <| post) <;> (intros; solve_by_elim [Sound.impl])
+
+instance : Sound (Wlp.assume (σ := σ) rq) where
+  inter := by intros; simp_all [actSimp]
+  impl := by intros; simp_all [actSimp]
+
+instance : Sound (Wlp.fresh (σ := σ) τ) where
+  inter := by intros; simp_all [actSimp]
+  impl := by intros; simp_all [actSimp]
+
+instance : Sound (Wlp.spec req ens) where
+  inter := by intros; simp_all [actSimp]
+  impl := by simp [actSimp]; intros; solve_by_elim
+
+instance (r : σ -> σ -> Prop) : Sound (r.toWlp) where
+  inter := by intros; simp_all [actSimp]
+  impl := by intros; simp_all [actSimp]
+
+instance : Sound (get (σ := σ)) where
+  inter := by intros; simp_all [get, getThe,MonadStateOf.get]
+  impl := by intros; simp_all [get, getThe,MonadStateOf.get]
+
+instance (s : σ) : Sound (set s : Wlp σ PUnit) where
+  inter := by intros; simp_all [set,MonadStateOf.set]
+  impl := by intros; simp_all [set,MonadStateOf.set]
+
+instance : Sound (modifyGet (σ := σ) f) where
+  inter := by intros; simp_all [modifyGet,MonadStateOf.modifyGet]
+  impl := by intros; simp_all [modifyGet,MonadStateOf.modifyGet]
+
+instance (act : Wlp σ ρ) [IsStateExtension σ σ'] [Sound act] :
+  Sound (monadLift act : Wlp σ' ρ) where
+  inter := by
+    intros; simp_all [monadLift, MonadLift.monadLift]
+    solve_by_elim [Sound.inter]
+  impl := by
+    intros; simp_all [monadLift, MonadLift.monadLift]
+    solve_by_elim [Sound.impl]
+
+end
